Start reworking clos_callProof for better compile_inc
Previously the incrementral compiler had as its state the same g as
the initial compiler, which carries around all of the generated code
in g. Using such a state for the incrementral compiler is terrible as
all of the already installed code would need to be kept forever.

My original plan was to split subg into two parts: one for the num_set
and one for the generated code. Howver, that turned out to require
essentially redoing the entire clos_call proof.

I opted for a more local approach whereby the incrementral compiler
has only the num_set in its state and, in the proof, recreates the
code part from the current code. This approach seems to work, but has
the slightly awkward case of specifying the code part for the limit
state.

compiler/backend/proofs/clos_callProofScript.sml
@@ -167,6 +167,24 @@ val wfg_def = Define`
     set (MAP FST (SND g)) = IMAGE SUC (domain (FST g)) ∧
     ALL_DISTINCT (MAP FST (SND g))`;
 
+val make_g_def = Define `
+  make_g d code =
+    if IMAGE SUC (domain d) ⊆ (FDOM code) then
+      SOME (d, MAP (\k. (FST k + 1, THE (FLOOKUP code (FST k + 1)))) (toAList d))
+    else NONE`;
+
+val ALL_DISTINCT_MAP_FST_ADD1 = prove(
+  ``!xs. ALL_DISTINCT (MAP (λk. FST k + 1n) xs) =
+         ALL_DISTINCT (MAP FST xs)``,
+  Induct \\ fs [MEM_MAP]);
+
+val make_g_wfg = store_thm("make_g_wfg",
+  ``make_g d code = SOME g ==> wfg g``,
+  rw [make_g_def,wfg_def] \\ fs [MAP_MAP_o,o_DEF]
+  \\ fs [ALL_DISTINCT_MAP_FST_ADD1,ALL_DISTINCT_MAP_FST_toAList]
+  \\ fs [EXTENSION,MEM_MAP,ADD1,EXISTS_PROD,MEM_toAList,domain_lookup]
+  \\ fs [PULL_EXISTS]);
+
 val recclosure_wf_def = Define`
   recclosure_wf loc fns ⇔
     every_Fn_SOME (MAP SND fns) ∧
@@ -269,11 +287,13 @@ val wfv_state_def = Define`
 val _ = temp_type_abbrev("calls_state",
           ``:num_set # (num, num # closLang$exp) alist``);
 
+val _ = temp_type_abbrev("abs_calls_state",``:num_set``);
+
 val correct_l_def = Define `
   correct_l l g <=> l = UNIV DIFF domain (FST g)`;
 
 val state_rel_def = Define`
-  state_rel g l (s:(calls_state # 'c,'ffi) closSem$state) (t:('c,'ffi) closSem$state) ⇔
+  state_rel g l (s:(abs_calls_state # 'c,'ffi) closSem$state) (t:('c,'ffi) closSem$state) ⇔
     (s.ffi = t.ffi) ∧
     (s.clock = t.clock) ∧
     (s.max_app = t.max_app) ∧
@@ -1443,7 +1463,7 @@ val wfv_v2l = Q.store_thm("wfv_v2l",
   \\ fs [wfv_def, v_to_list_def]);
 
 val do_app_thm = Q.store_thm("do_app_thm",
-  `case do_app op (REVERSE a) (r:(calls_state # 'c,'ffi) closSem$state) of
+  `case do_app op (REVERSE a) (r:(abs_calls_state # 'c,'ffi) closSem$state) of
       Rerr (Rraise _) => F
     | Rerr (Rabort e) =>
       (e = Rtype_error \/
@@ -1470,7 +1490,7 @@ val do_app_thm = Q.store_thm("do_app_thm",
   \\ reverse strip_tac
   THEN1
    (assume_tac (GEN_ALL simple_val_rel_do_app
-                |> INST_TYPE [alpha|->``:calls_state # 'c``])
+                |> INST_TYPE [alpha|->``:abs_calls_state # 'c``])
     \\ pop_assum (qspecl_then [`REVERSE v`,`REVERSE a`,
                 `v_rel g1 l1 t.code`,
                 `t`,`\s u. state_rel g1 l1 s u /\ u.code = t.code`,
@@ -1496,8 +1516,8 @@ val do_app_thm = Q.store_thm("do_app_thm",
     THEN1 (strip_tac \\ Cases_on `x = p` \\ fs [FAPPLY_FUPDATE_THM])
     THEN1 (strip_tac \\ Cases_on `x = p` \\ fs [FAPPLY_FUPDATE_THM]))
   \\ assume_tac (GEN_ALL simple_val_rel_do_app
-                 |> INST_TYPE [gamma|->``:calls_state # 'c``]
-                 |> INST_TYPE [alpha|->``:calls_state # 'c``])
+                 |> INST_TYPE [gamma|->``:abs_calls_state # 'c``]
+                 |> INST_TYPE [alpha|->``:abs_calls_state # 'c``])
   \\ pop_assum (qspecl_then [`REVERSE a`,`REVERSE a`,
                 `\v1 v2. wfv g1 l1 t.code v1 /\ v1 = v2`,
                 `r`,`\s1 s2. wfv_state g1 l1 t.code s1 /\ s1 = s2`,
@@ -1578,22 +1598,28 @@ val env_rel_Op_Install = prove(
   \\ qsuff_tac `!x. EXISTS (λx'. fv1 x x') e1 = fv x e1` \\ fs []
   \\ Induct_on `e1` \\ fs []);
 
-val compile_inc_def = Define `
-  compile_inc g (e,xs) =
-    let (ea, g') = calls [e] g in
-      (g', HD ea, TAKE (LENGTH (SND g') - LENGTH (SND g)) (SND g'))`;
-
 val syntax_ok_def = Define`
   syntax_ok x ⇔ every_Fn_SOME x ∧ every_Fn_vs_NONE x ∧ ALL_DISTINCT (code_locs x)`;
+
+val calls_acc = store_thm("calls_acc",
+  ``!xs d old res d1 aux.
+      calls xs (d, []) = (res, d1, aux) ==>
+      calls xs (d, old) = (res, d1, aux ++ old)``,
+  cheat (* routine proof? *));
+
+val compile_inc_def = Define `
+  compile_inc d (e,xs) =
+    let (ea, d1, new_code) = calls [e] (d,[]) in
+      (d1, HD ea, new_code)`;
 
 val co_ok_def = Define `
   co_ok code co g k <=>
     if k = 0 then T else
       let (cfg,exp,aux) = co 0 in
       let (g',exp',aux1) = compile_inc g (exp,aux) in
-        (∀x i. MEM x (code_locs [exp]) ∧ x ∉ domain (FST g') ==>
-               x ∉ domain (FST (FST (FST (co i))))) /\
-        code_includes (SND g') (code |++ aux1) /\
+        (∀x i. MEM x (code_locs [exp]) ∧ x ∉ domain g' ==>
+               x ∉ domain (FST (FST (co i)))) /\
+        DISJOINT (set (code_locs [exp])) (domain g) /\
         DISJOINT (FDOM code) (set (MAP FST aux1)) /\
         ALL_DISTINCT (MAP FST aux1) /\
         co_ok (code |++ aux1) (shift_seq 1 co) g' (k-1n)`
@@ -1603,12 +1629,10 @@ val code_inv_def = Define `
     s_code = FEMPTY /\
     s_cc = state_cc compile_inc t_cc /\
     t_co = state_co compile_inc s_co /\
+    (?full_g. make_g (FST (FST (s_co 0))) t_code = SOME full_g) /\
     (!k. co_ok t_code s_co (FST (FST (s_co 0))) k) /\
-    (!k n. k <= n ==> subg (FST (FST (s_co k))) (FST (FST (s_co n)))) /\
     (∀k. let (cfg,exp,aux) = s_co (k:num) in
-           DISJOINT (IMAGE SUC (set (code_locs [exp])))
-             (set (MAP FST (SND (FST cfg)))) /\
-           wfg (FST cfg) /\ aux = [] /\
+           aux = [] /\
            every_Fn_SOME [exp] /\
            every_Fn_vs_NONE [exp] /\
            ALL_DISTINCT (code_locs [exp]))`
@@ -1634,9 +1658,10 @@ val code_rel_state_rel_install = store_thm("code_rel_state_rel_install",
     DISJOINT (FDOM t.code) (set (MAP FST (SND progs))) ∧
     ALL_DISTINCT (MAP FST (SND progs)) /\
     t.compile cfg' progs = SOME (bytes,data,FST (shift_seq 1 t.compile_oracle 0)) /\
-    ?exp1 aux1 g5 exp5 aux5 other.
+    ?g4 exp1 aux1 g5 exp5 aux5 other.
       progs = (exp1,aux1) /\
-      calls [exp'] (FST cfg) = ([exp1],g5) /\
+      make_g (FST cfg) t.code = SOME g4 /\
+      calls [exp'] g4 = ([exp1],g5) /\
       state_rel g1 l1
        (r with
         <|compile_oracle := shift_seq 1 r.compile_oracle;
@@ -1645,59 +1670,74 @@ val code_rel_state_rel_install = store_thm("code_rel_state_rel_install",
         <|compile_oracle := shift_seq 1 t.compile_oracle;
           code := t.code |++ aux1|>) ∧
       code_inv (r.code |++ aux) r.compile (shift_seq 1 r.compile_oracle)
-        (t.code |++ aux1) t.compile (shift_seq 1 t.compile_oracle) /\
-      r.compile_oracle 1 = ((g5,other),exp5,aux5) /\
+               (t.code |++ aux1) t.compile (shift_seq 1 t.compile_oracle) /\
+      r.compile_oracle 1 = ((FST g5,other),exp5,aux5) /\
       t.code SUBMAP (t.code |++ aux1) /\
       code_includes (SND g5) (t.code |++ aux1)``,
-  Cases_on `calls [exp'] (FST cfg)` \\ fs []
+  strip_tac \\ fs [code_inv_def]
+  \\ Cases_on `calls [exp'] full_g` \\ fs []
   \\ imp_res_tac calls_sing \\ rveq \\ fs []
-  \\ PairCases_on `progs` \\ fs [] \\ strip_tac
+  \\ PairCases_on `progs` \\ fs []
   \\ fs [code_inv_def] \\ rfs []
+  \\ pop_assum mp_tac
   \\ pop_assum mp_tac
   \\ simp [Once state_co_def] \\ fs []
   \\ qpat_x_assum `_ = SOME _` mp_tac
   \\ simp [Once state_cc_def] \\ fs []
   \\ PairCases_on `cfg` \\ fs []
   \\ simp [Once compile_inc_def] \\ fs [] \\ rveq \\ fs []
-  \\ TOP_CASE_TAC \\ fs []
+  \\ simp [Once compile_inc_def] \\ fs [] \\ rveq \\ fs []
+  \\ `?x1 x2 x3. calls [exp'] (cfg0,[]) = (x1,x2,x3)` by metis_tac [PAIR] \\ fs []
+  \\ drule calls_acc
+  \\ disch_then (qspec_then `SND full_g` mp_tac)
+  \\ `(cfg0,SND full_g) = full_g` by (fs [make_g_def] \\ rveq \\ fs [])
+  \\ fs [] \\ pop_assum kall_tac
+  \\ simp [option_case_eq,pair_case_eq]
+  \\ ntac 4 strip_tac \\ rveq \\ fs []
   \\ rename [`t.compile cfg2 (output,_) = SOME xx`]
   \\ PairCases_on `xx` \\ fs []
   \\ fs [shift_seq_def] \\ rveq \\ fs []
-  \\ strip_tac \\ rveq \\ fs []
   \\ fs [compile_inc_def]
-  \\ strip_tac \\ rveq \\ fs []
   \\ simp [Once state_co_def] \\ fs []
-  \\ Cases_on `r.compile_oracle 1` \\ fs []
-  \\ rveq \\ fs []
+  \\ Cases_on `r.compile_oracle 1` \\ fs [] \\ rveq \\ fs []
   \\ rename [`r.compile_oracle 1 = ((r1,xx2),r2)`]
   \\ Cases_on `r2` \\ fs [compile_inc_def]
   \\ CONV_TAC (DEPTH_CONV PairRules.PBETA_CONV) \\ fs []
   \\ `aux = []` by (first_x_assum (qspec_then `0` mp_tac) \\ fs [])
   \\ fs [FUPDATE_LIST,state_co_def,state_rel_def]
-  \\ qabbrev_tac `aux1 = (TAKE (LENGTH (SND r1) − LENGTH cfg1) (SND r1))`
   \\ rewrite_tac [GSYM FUPDATE_LIST]
   \\ qpat_assum `!k. co_ok _ _ _ k` (qspec_then `1` mp_tac)
   \\ CONV_TAC (RATOR_CONV (SIMP_CONV std_ss [Once co_ok_def]))
   \\ fs [compile_inc_def] \\ strip_tac
-  \\ `t.code ⊑ t.code |++ aux1` by (match_mp_tac SUBMAP_FUPDATE_LIST \\ fs [])
-  \\ fs []
-  \\ reverse conj_tac THEN1
-   (rw [] \\ qpat_assum `!k. co_ok _ _ _ k` (qspec_then `k+1` mp_tac)
-    \\ CONV_TAC (RATOR_CONV (SIMP_CONV std_ss [Once co_ok_def]))
-    \\ fs [compile_inc_def,shift_seq_def])
-  \\ conj_tac THEN1
-   (match_mp_tac (GEN_ALL (MP_CANON LIST_REL_mono))
-    \\ first_assum(part_match_exists_tac (last o strip_conj) o concl) \\ rw[]
-    \\ match_mp_tac (GEN_ALL (MP_CANON OPTREL_MONO))
-    \\ first_assum(part_match_exists_tac (last o strip_conj) o concl) \\ fs []
-    \\ rw [] \\ match_mp_tac (GEN_ALL v_rel_SUBMAP) \\ asm_exists_tac \\ fs [])
-  THEN1
-   (match_mp_tac (GEN_ALL (MP_CANON fmap_rel_mono))
+  \\ `t.code ⊑ t.code |++ progs1` by (match_mp_tac SUBMAP_FUPDATE_LIST \\ fs [])
+  \\ fs [] \\ conj_tac THEN1
+   (conj_tac THEN1
+     (match_mp_tac (GEN_ALL (MP_CANON LIST_REL_mono))
+      \\ first_assum(part_match_exists_tac (last o strip_conj) o concl) \\ rw[]
+      \\ match_mp_tac (GEN_ALL (MP_CANON OPTREL_MONO))
+      \\ first_assum(part_match_exists_tac (last o strip_conj) o concl) \\ fs []
+      \\ rw [] \\ match_mp_tac (GEN_ALL v_rel_SUBMAP) \\ asm_exists_tac \\ fs [])
+    \\ match_mp_tac (GEN_ALL (MP_CANON fmap_rel_mono))
     \\ first_assum(part_match_exists_tac (last o strip_conj) o concl) \\ rw[]
     \\ Cases_on `x` \\ fs []
     \\ match_mp_tac (GEN_ALL (MP_CANON LIST_REL_mono))
     \\ first_assum(part_match_exists_tac (last o strip_conj) o concl) \\ rw[]
-    \\ match_mp_tac (GEN_ALL v_rel_SUBMAP) \\ asm_exists_tac \\ fs []))
+    \\ match_mp_tac (GEN_ALL v_rel_SUBMAP) \\ asm_exists_tac \\ fs [])
+  \\ conj_tac
+  THEN1 (fs [make_g_def] \\ cheat (* easy? *))
+  \\ conj_tac
+  THEN1
+   (rw [] \\ qpat_assum `!k. co_ok _ _ _ k` (qspec_then `k+1` mp_tac)
+    \\ CONV_TAC (RATOR_CONV (SIMP_CONV std_ss [Once co_ok_def]))
+    \\ fs [compile_inc_def,shift_seq_def])
+  \\ fs [make_g_def] \\ rveq \\ fs [code_includes_def]
+  \\ fs [flookup_update_list_some,ALOOKUP_APPEND,option_case_eq]
+  \\ fs [alookup_distinct_reverse]
+  \\ rw [] \\ fs []
+  \\ imp_res_tac ALOOKUP_MEM
+  \\ fs [MEM_MAP] \\ rename [`MEM kk _`]
+  \\ PairCases_on `kk` \\ rveq \\ fs []
+  \\ fs [MEM_toAList,SUBSET_DEF,PULL_EXISTS,ADD1,FLOOKUP_DEF,domain_lookup])
   |> GEN_ALL;
 
 val fv_GENLIST_Var_alt = store_thm("fv_GENLIST_Var_alt",
@@ -1717,7 +1757,7 @@ val env_rel_env_exists = store_thm("env_rel_env_exists",
 
 val includes_state_def = Define `
   includes_state g1 s_compile_oracle <=>
-    ?k:num. FST (FST (s_compile_oracle k)) = g1`;
+    ?k:num. FST (FST (s_compile_oracle k)) = FST g1`;
 
 val evaluate_includes_state = store_thm("evaluate_includes_state",
   ``!xs env s res s1 g1.
@@ -1810,7 +1850,12 @@ val calls_correct = Q.store_thm("calls_correct",
       code_inv s.code s.compile s.compile_oracle
                t.code t.compile t.compile_oracle ∧
       result_rel (LIST_REL (v_rel g l t.code)) (v_rel g l t.code) res res')`,
+
   ho_match_mp_tac evaluate_ind
+  \\ ntac 7 (conj_tac >- cheat)
+  \\ reverse conj_tac THEN1 cheat
+
+(*
   \\ conj_tac >- (
     rw[]
     \\ qexists_tac`0`
@@ -2321,8 +2366,9 @@ val calls_correct = Q.store_thm("calls_correct",
     \\ qexists_tac `ck+ck'` \\ fs [AC ADD_COMM ADD_ASSOC]
     \\ fs [evaluate_def])
   (* Op *)
-  \\ conj_tac >- (
-    fs [evaluate_def,calls_def] \\ rw []
+  \\ conj_tac >- ( *)
+
+    \\ fs [evaluate_def,calls_def] \\ rw []
     \\ pairarg_tac \\ fs [] \\ rw []
     \\ fs [evaluate_def]
     \\ Cases_on `evaluate (xs,env,s)` \\ fs []
@@ -2419,6 +2465,7 @@ val calls_correct = Q.store_thm("calls_correct",
     \\ drule code_rel_state_rel_install
     \\ fs [shift_seq_def]
     \\ rpt (disch_then drule) \\ strip_tac
+    \\ imp_res_tac make_g_wfg
     \\ `t.clock <> 0` by fs [state_rel_def] \\ fs []
     \\ fs [state_rel_def,FUPDATE_LIST]
     \\ first_x_assum drule
@@ -2452,16 +2499,31 @@ val calls_correct = Q.store_thm("calls_correct",
       \\ simp [includes_state_def] \\ strip_tac
       \\ qpat_x_assum `_ = (res,s')` assume_tac
       \\ drule evaluate_code \\ rw [] \\ fs [shift_seq_def]
-      \\ rpt (first_x_assum (qspecl_then [`1`,`k+n+1`] mp_tac)) \\ fs [])
+      \\ rpt (first_x_assum (qspecl_then [`1`,`k+n+1`] mp_tac)) \\ fs []
+      \\ cheat)
     \\ fs [correct_l_def]
     \\ fs [SUBSET_DEF]
     \\ fs [code_inv_def]
-    \\ qpat_x_assum `∀k. co_ok t.code r.compile_oracle (FST cfg) k` mp_tac
+    \\ `FST cfg = FST g4` by (fs [make_g_def] \\ rveq \\ fs []) \\ fs []
+    \\ qpat_x_assum `∀k. co_ok t.code r.compile_oracle (FST g4) k` mp_tac
     \\ disch_then (qspec_then `1` mp_tac)
     \\ once_rewrite_tac [co_ok_def] \\ fs [compile_inc_def]
     \\ qpat_x_assum `includes_state g1 r.compile_oracle` mp_tac
     \\ simp [includes_state_def] \\ strip_tac \\ rveq
-    \\ metis_tac [])
+    \\ `?y1 y2 y3. (calls [exp'] (FST g4,[])) = (y1,y2,y3)` by metis_tac [PAIR]
+    \\ drule calls_acc
+    \\ disch_then (qspec_then `SND g4` mp_tac) \\ fs []
+    \\ strip_tac \\ rveq \\ fs []
+    \\ rpt strip_tac THEN1 fs [wfg_def,DISJOINT_IMAGE_SUC]
+    \\ first_x_assum drule
+    \\ disch_then drule \\ fs []
+    \\ qpat_x_assum `includes_state g1 s'.compile_oracle` mp_tac
+    \\ simp [includes_state_def] \\ strip_tac
+    \\ qpat_x_assum `_ = (res,s')` assume_tac
+    \\ drule evaluate_code \\ rw [] \\ fs [shift_seq_def]
+    \\ metis_tac []
+
+(*
   (* Fn *)
   \\ conj_tac >- (
     rw[evaluate_def]
@@ -2980,7 +3042,8 @@ val calls_correct = Q.store_thm("calls_correct",
          \\ imp_res_tac evaluate_mono \\ fs [])
       \\ fs []
       \\ strip_tac \\ rveq
-      \\ drule (Q.GEN`s`pure_correct |> INST_TYPE [``:'c``|->``:calls_state # 'c``])
+      \\ drule (Q.GEN`s`pure_correct
+                |> INST_TYPE [``:'c``|->``:abs_calls_state # 'c``])
       \\ disch_then(qspec_then`r`mp_tac)
       \\ simp[]
       \\ reverse BasicProvers.TOP_CASE_TAC \\ fs[]
@@ -3648,7 +3711,7 @@ val calls_correct = Q.store_thm("calls_correct",
   \\ qmatch_assum_abbrev_tac `closSem$evaluate (_,_,(_ with clock := ck11)) = _`
   \\ qmatch_goalsub_abbrev_tac `_ with clock := ck22`
   \\ qsuff_tac `ck11 = ck22` \\ rw [] \\ fs []
-  \\ unabbrev_all_tac \\ fs []);
+  \\ unabbrev_all_tac \\ fs [] *));
 
 val code_locs_calls_list = Q.prove(`
   ∀ls n tr i. code_locs (MAP SND (calls_list tr i n ls)) = []`,
@@ -3723,12 +3786,12 @@ val calls_code_locs_ALL_DISTINCT = Q.store_thm("calls_code_locs_ALL_DISTINCT",
 val extra_code_assum_def = Define `
   extra_code_assum prog g0 co =
     ∀n m. MEM n (code_locs prog) ∧ n ∉ domain g0 ⇒
-          n ∉ domain (FST (FST (FST (co m))))`;
+          n ∉ domain (FST (FST (co m)))`;
 
 val semantics_calls = Q.store_thm("semantics_calls",
   `semantics (ffi:'ffi ffi_state) max_app FEMPTY co cc x <> Fail ==>
    compile T x = (y,g0,aux) /\ every_Fn_SOME x ∧ every_Fn_vs_NONE x /\
-   ALL_DISTINCT (code_locs x) /\ FST (FST (co 0)) = (g0,aux) /\
+   ALL_DISTINCT (code_locs x) /\ FST (FST (co 0)) = g0 /\
    extra_code_assum x g0 co /\
    code_inv FEMPTY cc co (FEMPTY |++ aux) cc1 co1 ==>
    semantics (ffi:'ffi ffi_state) max_app (FEMPTY |++ aux) co1 cc1 y =
@@ -3743,38 +3806,36 @@ val semantics_calls = Q.store_thm("semantics_calls",
   \\ rpt (disch_then drule) \\ fs [EVAL ``wfg (LN,[])``]
   \\ disch_then (qspecl_then [`[]`,
       `initial_state ffi max_app (FOLDL $|+ FEMPTY aux) co1 cc1 k`,
-      `UNIV DIFF domain (FST (FST (FST (s2.compile_oracle 0))))`,
-      `FST (FST (s2.compile_oracle 0))`] mp_tac)
+      `UNIV DIFF domain (FST (FST (s2.compile_oracle 0)))`,
+      `THE (make_g ((FST (FST (s2.compile_oracle 0)))) s2.code)`] mp_tac)
   \\ simp []
-  \\ `wfg (g0,aux)` by
+  \\ `wfg (FST (FST (co 0)),aux)` by
    (match_mp_tac calls_wfg
     \\ asm_exists_tac \\ fs []
     \\ EVAL_TAC \\ fs [])
+  \\ `?rest.
+        make_g (FST (FST (s2.compile_oracle 0))) s2.code =
+          SOME (FST (FST (s2.compile_oracle 0)),rest)` by cheat
+  \\ fs []
   \\ impl_tac THEN1
    (rpt conj_tac
     \\ fs [env_rel_def,state_rel_def,initial_state_def,code_includes_def]
     \\ fs [correct_l_def]
     THEN1 (fs [wfv_state_def,initial_state_def,FEVERY_DEF,code_inv_def])
     THEN1
-     (drule evaluate_code \\ rw [] \\ fs []
-      \\ fs [code_inv_def,shift_seq_def]
-      \\ first_x_assum (qspecl_then [`0`,`n`] mp_tac) \\ fs [])
+     (imp_res_tac make_g_wfg \\ fs [wfg_def,subg_def] \\ cheat (* subg *))
     THEN1
      (fs [SUBSET_DEF]
       \\ drule evaluate_code \\ strip_tac
       \\ fs [shift_seq_def,extra_code_assum_def])
     THEN1 (fs [IN_DISJOINT,IN_DIFF] \\ metis_tac [])
-    THEN1
-     (drule evaluate_code \\ rw [] \\ fs []
-      \\ fs [code_inv_def,shift_seq_def]
-      \\ rpt (first_x_assum (qspecl_then [`n`] mp_tac)) \\ fs []
-      \\ Cases_on `co n` \\ fs [] \\ PairCases_on `r` \\ fs [])
+    THEN1 (imp_res_tac make_g_wfg \\ fs [])
     THEN1
      (full_simp_tac std_ss [GSYM FUPDATE_LIST]
       \\ rpt strip_tac
       \\ match_mp_tac mem_to_flookup
       \\ fs [ALOOKUP_MEM]
-      \\ `aux = SND (g0,aux)` by fs []
+      \\ `aux = SND (FST (FST (co 0)),aux)` by fs []
       \\ pop_assum (fn th => once_rewrite_tac [th])
       \\ match_mp_tac calls_ALL_DISTINCT
       \\ asm_exists_tac \\ fs [])
@@ -3793,7 +3854,7 @@ val semantics_compile = Q.store_thm("semantics_compile",
   `semantics ffi max_app FEMPTY co cc x ≠ Fail ∧
    compile do_call x = (y,g1,aux) ∧
    (if do_call then
-    syntax_ok x ∧ FST (FST (co 0)) = (g1,aux) ∧
+    syntax_ok x ∧ FST (FST (co 0)) = g1 ∧
     extra_code_assum x g1 co /\
     code_inv FEMPTY cc co (FEMPTY |++ aux) cc1 co1
     else cc = state_cc (CURRY I) cc1 ∧
